

# NLP hw3

Huizhen Jin [hj1314]

October 2025

## 1 Recurrent Neural Network

### RNN Derivatives

1 The per-example cross-entropy loss for the classification task is defined as:

$$\ell(y, \mathbf{p}_T) = - \sum_{i=1}^k y[i] \cdot \log(p_T[i])$$

Since  $y \in \{0, 1\}^k$  is a one-hot vector, only the true label contributes to the sum. Let  $c$  be the index such that  $y[c] = 1$ . Then the expression simplifies to:

$$\ell(y, \mathbf{p}_T) = -\log(p_T[c])$$

2(a) Let  $w = W_{hh}[i, j]$  be the  $(i, j)$ -th entry of the recurrent weight matrix. We treat  $h_{i-1}$  as constant and compute the immediate gradient  $\frac{\partial h_i^+}{\partial w}$  using the chain rule:

$$\frac{\partial h_i^+}{\partial W_{hh}[i, j]} = \sigma'(z_i[i]) \cdot h_{i-1}[j]$$

where:

- $z_i = W_{hh}h_{i-1} + W_{ih}x_i + b_h$  is the pre-activation input to the nonlinearity at time step  $i$ ,
- $\sigma(\cdot)$  is the tanh activation function, and
- $\sigma'(z_i[i]) = 1 - \tanh^2(z_i[i])$

2(b) We are asked to expand the gradient vector  $\frac{\partial h_t}{\partial h_i}$  using the chain rule, expressing it as a product of partial derivatives between successive hidden states.

Using the chain rule, we have:

$$\frac{\partial h_t}{\partial h_i} = \frac{\partial h_t}{\partial h_{t-1}} \cdot \frac{\partial h_{t-1}}{\partial h_{t-2}} \cdot \dots \cdot \frac{\partial h_{i+1}}{\partial h_i} = \prod_{j=i+1}^t \frac{\partial h_j}{\partial h_{j-1}}$$

This expression captures how the hidden state at time  $i$  influences the final hidden state  $h_t$  through all intermediate steps from  $i+1$  to  $t$ .

3 We are asked to write the Jacobian matrix  $\frac{\partial h_{i+1}}{\partial h_i}$  by applying the rules of differentiation. Recall that the hidden state is updated as:

$$h_{i+1} = \sigma(W_{hh}h_i + W_{ih}x_{i+1} + b_h)$$

Let  $z_{i+1} = W_{hh}h_i + W_{ih}x_{i+1} + b_h$ , so that  $h_{i+1} = \sigma(z_{i+1})$ . Applying the chain rule:

$$\frac{\partial h_{i+1}}{\partial h_i} = \frac{\partial \sigma(z_{i+1})}{\partial z_{i+1}} \cdot \frac{\partial z_{i+1}}{\partial h_i}$$

We now compute each term:

- $\frac{\partial z_{i+1}}{\partial h_i} = W_{hh}$
- $\frac{\partial \sigma(z_{i+1})}{\partial z_{i+1}} = \text{diag}(\sigma'(z_{i+1}))$ , since the activation function is applied element-wise

Therefore, the full Jacobian is:

$$\frac{\partial h_{i+1}}{\partial h_i} = \text{diag}(\sigma'(z_{i+1})) \cdot W_{hh}$$

## Bounding Gradient Norm

1 Given the Jacobian matrix derived earlier,

$$\frac{\partial h_i}{\partial h_{i-1}} = \text{diag}(\sigma'(z_i)) \cdot W_{hh},$$

we can apply the submultiplicative property of the spectral norm:

$$\|AB\|_2 \leq \|A\|_2 \cdot \|B\|_2$$

to obtain the following bound:

$$\left\| \frac{\partial h_i}{\partial h_{i-1}} \right\|_2 \leq \|\text{diag}(\sigma'(z_i))\|_2 \cdot \|W_{hh}\|_2$$

Since the activation function  $\sigma(\cdot) = \tanh(\cdot)$  satisfies  $\sigma'(z_i) \leq 1$  for all  $z_i$ , we also have the looser upper bound:

$$\left\| \frac{\partial h_i}{\partial h_{i-1}} \right\|_2 \leq \|W_{hh}\|_2$$

2 We can express the derivative of the hidden state at time  $t$  with respect to that at time  $i$  as a product of Jacobians:

$$\frac{\partial h_t}{\partial h_i} = \prod_{k=i+1}^t \frac{\partial h_k}{\partial h_{k-1}}$$

Taking the spectral norm on both sides and applying the submultiplicative property of matrix norms gives:

$$\left\| \frac{\partial h_t}{\partial h_i} \right\|_2 \leq \prod_{k=i+1}^t \left\| \frac{\partial h_k}{\partial h_{k-1}} \right\|_2 \leq \prod_{k=i+1}^t (\|\text{diag}(\sigma'(z_k))\|_2 \cdot \|W_{hh}\|_2)$$

Since the derivative of the tanh activation satisfies  $\sigma'(z) \leq 1$ , each  $\|\text{diag}(\sigma'(z_k))\|_2 \leq 1$ . Hence, the gradient norm is bounded by:

$$\left\| \frac{\partial h_t}{\partial h_i} \right\|_2 \leq \|W_{hh}\|_2^{(t-i)}$$

If  $\|W_{hh}\|_2 < 1$ , this bound decays exponentially, leading to **vanishing gradients**. If  $\|W_{hh}\|_2 > 1$ , it grows exponentially, causing **exploding gradients**. Only when  $\|W_{hh}\|_2 \approx 1$  do gradients remain stable during back-propagation through time.